Main.lean
@@ -2,8 +2,7 @@ import VersoManual
 import FPCourse
 open Verso.Genre.Manual
 def main := manualMain (%doc FPCourse) (config := {
-  htmlDepth := 2
-  rootTocDepth := .some 2
-  sectionTocDepth := .some 2
-  
+  htmlDepth := 1
+  rootTocDepth := .some 1
+  sectionTocDepth := .some 1
 })
